#Project #PAI 

We have that: $$\begin{align}0&=\frac{d}{da}\mathbb{E}[\ell(y,a)|x]\\&=c_{1}\frac{d}{da}\int_{a}^{\infty} (y-a)^{2} p(y|x)\, dy+c_{2} \frac{d}{da}\int_{-\infty}^{a} (a-y)^{2} p(y|x)\, dy \\&=2\left(- c_{1}\int_{a}^{\infty} (y-a) p(y|x)\, dy+c_{2}\int_{-\infty}^{a} (a-y)p(y|x) \, dy   \right)\\&=2\left(ac_{1}(1-F(a))+c_{2}aF(a)- c_{1}\int_{a}^{\infty} y p(y|x)\, dy-c_{2}\int_{-\infty}^{a} yp(y|x) \, dy   \right)\\&=2\left(ac_{1}(1-F(a))+c_{2}aF(a)- \frac{c_{1}}{\sqrt{ 2\pi\sigma^{2} }}\int_{a}^{\infty} y \exp \left( -\frac{(y-\mu)^2}{2\sigma^{2}} \right) \, dy-\frac{c_{2}}{\sqrt{ 2\pi\sigma^{2} }}\int_{-\infty}^{a} y\exp \left( -\frac{(y-\mu)^2}{2\sigma^{2}} \right) \, dy   \right)\end{align}$$where: $$\begin{align} \frac{1}{\sqrt{ 2\pi\sigma^{2}}}\int_{a}^{\infty} y \exp \left( -\frac{(y-\mu)^2}{2\sigma^{2}} \right) \, dy&=\frac{1}{\sqrt{ 2\pi\sigma^{2}}}\int_{a}^{\infty} y\exp \left( -\frac{y^2}{2\sigma^{2}} \right) \, dy+\mu(1-F(a))\\&=\frac{2\sigma^{2}}{\sqrt{ 2\pi\sigma^{2}}} \int_{\frac{a}{\sqrt{ 2\sigma^{2} }}}^{\infty} y\exp \left( -y^{2}\right) \, dy+\mu(1-F(a))\\&={\sqrt{ \frac{\sigma^{2}}{2\pi}}}\exp \left( -\frac{a^{2} }{2\sigma^{2}}   \right) +\mu(1-F(a))\end{align}$$ and: $$\begin{align} \frac{1}{\sqrt{ 2\pi\sigma^{2}}}\int_{-\infty}^{a} y \exp \left( -\frac{(y-\mu)^2}{2\sigma^{2}} \right) \, dy&=\frac{1}{\sqrt{ 2\pi\sigma^{2}}}\int_{-\infty}^{a} y\exp \left( -\frac{y^2}{2\sigma^{2}} \right) \, dy+\mu F(a)\\&=\frac{2\sigma^{2}}{\sqrt{ 2\pi\sigma^{2}}} \int_{-\infty}^{a/\sqrt{ 2\sigma^{2} }} y\exp \left( -y^{2}\right) \, dy+\mu F(a)\\&=-{\sqrt{ \frac{\sigma^{2}}{2\pi}}}\exp \left( -\frac{a^{2} }{2\sigma^{2}}   \right) +\mu F(a)\end{align}$$Hence, $$\begin{align}0&=ac_{1}(1-F(a))+c_{2}aF(a)+(c_{2}-c_{1})k\exp \left( -\frac{a^{2}}{2\sigma^{2}} \right) -c_{1}\mu(1-F(a))-c_{2}\mu F(a)\\&=ac_{1}+a(c_{2}-c_{1})F(a)+(c_{2}-c_{1})k\exp \left( -\frac{a^{2}}{2\sigma^{2}} \right) -c_{1}\mu-(c_{2}-c_{1})\mu F(a)\\&=ac_{1}+(a-\mu)(c_{2}-c_{1})F(a)+(c_{2}-c_{1})k\exp \left( -\frac{a^{2}}{2\sigma^{2}} \right) -c_{1}\mu\end{align}$$

---
##### Attempt 2
$$\begin{align}\mathbb{E}[\ell(y,a)|x]&=c_{1}\int_{-\infty}^{a} (y-a)^{2} p(y|x)\, dy+c_{2}\int_{a}^{\infty} (y-a)^{2} p(y|x)\, dy\\&=c_{1}\mathbb{E}[(y-a)^{2}|x]+(c_{2}-c_{1})\int_{a}^{\infty} (y-a)^{2}p(y|x) \, dy\\&=c_{1}\mathbb{E}[y^{2}|x]-2c_{1}\mu a+c_{1}a^{2}+(c_{2}-c_{1})\int_{a}^{\infty} (y-a)^{2}p(y|x) \, dy  \end{align}$$Hence, $$\begin{align}0=\frac{d}{da}\mathbb{E}[\ell(y,a)|x]&=-2c_{1}\mu+2c_{1}a-2(c_{2}-c_{1})\int_{a}^{\infty} (y-a) p(y|x)\, dy\\&=-2c_{1}\mu+2c_{1}a-2(c_{2}-c_{1})\left( \int_{a}^{\infty} y p(y|x)\, dy-a(1-F(a)) \right) \\&=-2c_{1}\mu+2c_{1}a-2(c_{2}-c_{1})\left( {\sqrt{ \frac{\sigma^{2}}{2\pi}}}\exp \left( -\frac{a^{2} }{2\sigma^{2}}   \right) -(a-\mu)(1-F(a)) \right) \\&=(a-\mu)\left( 2c_{1}+2(c_{2}-c_{1})(1-F(a)) \right) -2(c_{2}-c_{1}) {\sqrt{ \frac{\sigma^{2}}{2\pi}}}\exp \left( -\frac{a^{2} }{2\sigma^{2}}   \right)\end{align}$$

---