#Definition #Algebra 

> [!definition]
> Let $M,N,P$ be $R$-[[Module|modules]]. 
> 1. A map $\alpha:M\times N\to P$ is called ***bilinear*** if $\alpha(m,\cdot):N\to P$ and $\alpha(\cdot,n):M\to P$ are $R$-linear for all $m\in M,n\in N$.
> 2. A ***tensor product of $M$ and $N$ over $R$*** is an $R$-module $M\otimes_{R} N$ together with a bilinear map $\tau:M\times N\to M\otimes N$ s.t. 
> 	1. **universal property**: for every bilinear map $\alpha:M\times N\to P$, there exists a unique linear map $\varphi:M\otimes N\to P$ s.t. $\alpha=\varphi \circ \tau$.
> 
> The elements in $M\otimes N$ are called ***tensors*** and for $(m,n)\in M\times N$, $m\otimes n:= \tau(m,n)$. 

- **Remark**: By the definition, we have that $\text{Bilinear}(M\times N, P)\cong \text{Hom}(M\otimes N,P)$, i.e. they are bijective.
- **Related definition**: Tensors in $M\otimes N$ of the form $m\otimes n$ are called ***pure/monomial***. Any tensor can be written as a linear combination of pure tensors. 

---
##### Properties
> [!lemma] Theorem 1 (Uniqueness and Existence of Tensor Products)
> Let $M,N$ be $R$-modules. Then,
> 1. **Existence**: there exists a tensor product $M\otimes N$.
> 2. **Uniqueness**: the tensor product is unique up to isomorphism, i.e. if $(M\otimes N, \tau)$ and $(M\otimes' N,\tau')$ are two tensor products of $M,N$, then there is a unique $R$-isomorphism $\varphi:M\otimes N\to M\otimes'N$ s.t. $\tau'=\varphi\circ \tau$.

> [!proof]-
> We have that:
> 1. As $\tau':M\times N\to M\otimes'N$ is a bilinear map, by the universal property, there exists a unique linear map $\varphi:M\otimes N\to M\otimes'N$ s.t. $\tau'=\varphi \circ \tau$. The same way we get a unique linear map $\psi:M\otimes' N\to M\otimes N$ with $\tau=\psi \circ \tau'$.
>    
>    By applying the universal property again on $\tau$, we have a unique linear map $\alpha:M\otimes N\to M\otimes N$ s.t. $\tau= \alpha \circ \tau$. As we have that: $$\tau = \psi \circ  \varphi \circ  \tau, \quad \tau=\text{id} \circ  \tau$$By uniqueness, $\alpha=\text{id}=\psi \circ \varphi$ and similarly $\varphi \circ \psi=\text{id}$. Hence, $\varphi$ is an isomorphism. 
> 2. Let $F$ be the $R$-module of all finite formal linear combinations of $M\times N$, i.e. $$F:=\left\{  \sum_{i=1}^{n}a_{i}(m_{i},n_{i}) :n\in \mathbb{N}, a_{i}\in R, (m_{i},n_{i})\in M\times N  \right\}$$Now, let $G$ be a submodule generated by: 
> 	1. $(m_{1}+m_{2},n)-(m_{1},n)-(m_{2},n)$
> 	2. $(m,n_{1}+n_{2})-(m,n_{1})-(m,n_{2})$
> 	3. $(am,n)-a(m,n)$
> 	4. $(m,an)-a(m,n)$
> 	
> 	for all $m,m_{1},m_{2}\in M,n,n_{1},n_{2}\in N,a\in R$. Now, set $M\otimes N:= F /G$. Then, the map: $$\tau:M\times N\to M\otimes N,\quad (m,n)\mapsto \overline{(m,n)}$$ is a bilinear map. We claim that $M\otimes N$ with $\tau$ is a tensor product of $M,N$ over $R$. Let $\alpha:M\times N\to P$ be a $R$-bilinear map. Then, define $\varphi:M\otimes N\to P$ by setting $\varphi(\overline{(m,n)}):=\alpha(m,n)$ and extending it by linearity. 
> 	
> 	Since $\alpha$ is bilinear, $\varphi$ is well-defined and $\alpha=\varphi \circ \tau$. It is also clear that this is the unique choice that makes this possible. This proves the claim.
---
> [!lemma] Proposition 2
> If $\{ v_{i} \}_{i}$ is a basis of $V$ and $\{ w_{j} \}_{j}$ is a basis of $W$, $\{ v_{i}\otimes w_{j} \}_{i,j}$ is a basis of $V\otimes W$. 

> [!proof]-
> Clearly $\{ v_{i}\otimes w_{j} \}$ spans $V\otimes W$ by definition. To see the linear independence, let $e_{ij}:V\otimes W\to K$ be s.t. $e_{ij}(v_{i}\otimes w_{j})=1$ and vanishes on any other basis tensor. 
> 
> Assume that $A:=\sum_{i,j}^{}a_{ij}(v_{i}\otimes w_{j})=0$. Then, $e_{ij}(A)=a_{ij}=0$ for all $i,j$.
---
##### Examples

> [!h] Example 1
> Let $V$ be a finite-dimensional vector space. Then, $$\begin{array}{cccc} {J:}&{V^{*}\otimes W}&\to&{\text{Hom}(V,W)}\\&{f\otimes w} &\mapsto & {v\mapsto f(v)w} \end{array}{}$$is an isomorphism.

> [!proof]-
> First we show that $J(f\otimes w)$ is well-defined. $$J(f\otimes w)(v_{1}+v_{2})=f(v_{1})w+f(v_{2})w=J(f\otimes w)v_{1}+J(f\otimes w)v_{2}$$$$J(f\otimes w)(av)=af(v)w=aJ(f\otimes w)v$$
> If $J(f\otimes w)=0$, then either $f=0$ or $w=0$. Therefore, $\text{ker }J=(0)$. Further, for $A\in \text{Hom}(V,W)$, let $f_{i}$ be the basis of $V^{*}$. Then, consider $\sum_{i}^{}f_{i}\otimes A(v_{i})$. $$J\left( \sum_{i}^{}f_{i}\otimes A(v_{i}) \right)(v)=\sum_{i}^{}f_{i}(v)A(v_{i})=A\left( \sum_{i}^{}f_{i}(v)v_{i} \right)=A(v) $$
---
> [!h] Example 2 (Symmetric and Exterior Power)
> Let $V$ be a $K$-vector space. We define: $$S^nV:=V^{\otimes n} / \braket{ T-s(T) :T\in V^{\otimes }n ,s\in \text{Trans}} $$i.e. where $s$ is a transposition. If $\{ v_{i} \}_{i}$ is a basis of $V$, then $\{ v_{i_{1}}\otimes\dots \otimes v_{i_{n}}:i_{1}\leq\dots\leq i_{n} \}$ is the basis of $S^nV$ with dimension ${m+n-1\choose n}$ for $\text{dim} V=m$.
> 
> Similarly, for: $$\land^nV:=V^{\otimes n} / \braket{ s(T)=T  } $$we have $\{ v_{i_{1}}\otimes\dots \otimes v_{i_{n}}:i_{1}<\dots<i_{n} \}$ as a basis with dimension $m \choose n$.
---
