#### Problem 1
1. Let $M\in \mathbb{R}^{n,n}$. Let $u_{1},\dots,u_{n},v_{1},\dots,v_{n}\in \mathbb{R}^{2n}$ be unit vectors. Then, we define $U:=(u_{1},\dots,u_{n})\in \mathbb{R}^{2n,n}$ and $V:=(v_{1},\dots,v_{n})\in \mathbb{R}^{2n,n}$. We define: $$X:=(U,V)\in \mathbb{R}^{2n,2n},\quad Z:=X^\top X\in \mathbb{R}^{2n,2n}$$Then, $Z$ is symmetric positive semidefinite as all matrices of this form are. Further, $$Z_{ii}=\sum_{j\in [2n]}^{}X_{ji}^2=1,\quad \forall i\in[2n]$$as $X$ only has unit columns. Now, notice that: $$\left\langle Z , \begin{bmatrix}0&M\\0&0\end{bmatrix} \right\rangle =\sum_{i,j\in[n]}^{}M_{ij} Z_{i,n+j}=\sum_{i,j\in[n]}^{}M_{ij} \sum_{k\in[2n]}^{}u_{i}(k)v_{j}(k)=\sum_{i,j\in[n]}^{}M_{ij} \braket{ u_{i} , v_{j} } $$Therefore, $f_{=}(M)\leq \left\| M \right\|_{G}$.
2. Let $M\in \mathbb{R}^{n,n}$. Let $X\in \mathbb{R}^{2n,2n}$ be a symmetric positive semidefinite matrix s.t. $\text{diag}(X)=I_{2n}$. Then, there exists a Cholesky decomposition s.t. $X=L^\top L$ with $L\in \mathbb{R}^{2n,2n}$. Let $(u_{1},\dots,u_{n},v_{1},\dots,v_{n}):= L$. We have that for any $i\in[n]$, $$1=(L^\top L)_{ii}=\left\| u_{i} \right\| ^{2}$$and similarly $\left\| v_{i} \right\|=1$. Now, we have: $$\left\langle X,\begin{bmatrix}0&M\\0&0\end{bmatrix}\right\rangle =\braket{ X_{1,2} , M } =\sum_{i,j\in[n]}^{}M_{ij}\braket{ u_{i} , v_{j} } $$and $\left\| M \right\|_{G}\leq f_{=}(M)$.
3. Let $M\in \mathbb{R}^{n,n}$. By definition we have that $f_{=}(M)\leq f_{\leq }(M)$. Conversely, let $u_{1},\dots,u_{n},v_{1},\dots,v_{n}\in \mathbb{R}^{2n}$ s.t. $\left\| u_{i} \right\|,\left\| v_{j} \right\|\leq 1$. 
   
   If none of the $u_{i},v_{j}=0$ then define $u'_{i}:= u_{i} / \left\| u_{i} \right\|$ and $v'_{j}:= v_{j} / \left\| v_{j} \right\|$. We then have: $$\sum_{i,j\in[n]}M_{ij}\braket{ u'_{i} , v'_{j} } =\sum_{i,j\in[n]} M_{ij}\braket{ u_{i} , v_{j} }\cdot  \frac{1}{\left\| u_{i} \right\| \left\| v_{j} \right\|} \geq\sum_{i,j\in[n]}M_{ij}\braket{ u_{i} , v_{j} }$$Now notice that for a fixed $k$, $$\sum_{i,j\in[n]}^{}M_{ij}\braket{ u_{i} , v_{j} } =\sum_{i\neq k}^{}\sum_{j\in[n]}^{}M_{ij}\braket{ u_{i} , v_{j} } +\sum_{j\in[n]}^{}M_{kj}\braket{ u_{k} , v_{j} } $$Then, we have $\sum_{j\in[n]}^{}M_{kj}\braket{ u_{k} , v_{j} }=u_{i}^\top\left(  \sum_{j\in[n]}^{}M_{kj}v_{j} \right)$. Therefore, if $u_{k}=0$, then there always exist a non-zero $u'_{k}$ with $\left\| u'_{k} \right\|\leq 1$ s.t. $\sum_{j\in[n]}^{}M_{kj}\braket{ u_{k}' , v_{j} }\geq 0$. This shows that we can reduce this case to the first, where none of the $u_{i},v_{j}=0$. 
   
   Therefore, this shows that $f_{=}(M)\geq f_{\leq }(M)$.

---
#### Problem 2
1. Notice that: $$\braket{ x^{>\tau} , Ay^{\leq \tau} } =\sum_{k,\ell\in[n]}^{}x^{> \tau}_{k}A_{k\ell} y^{\leq \tau}_{\ell}=\braket{ (w_{1}w_{1}^\top)_{1,2} , A }=\left\langle w_{1}w_{1}^\top , \begin{bmatrix}0&A\\0&0\end{bmatrix} \right\rangle  $$Hence, similarly, $$\braket{ x^{>\tau} , Ay^{\leq \tau} } +\braket{ x^{\leq\tau} , Ay^{> \tau} } +\braket{ x^{>\tau} , Ay^{> \tau} } =\left\langle w_{1}w_{1}^\top + w_{2}w_{2}^\top + w_{3}w_{3}^\top , \begin{bmatrix}0&A\\0&0\end{bmatrix} \right\rangle $$ Now, as $x_{i},y_{i}$ they are all identically distributed, $$W_{ii}=\mathbb{E}[2(x_{i}^{>\tau})^{2}+(x_{i}^{\leq\tau})^{2}]$$$$\mathbb{E}[w_{1}w_{1}^\top]_{ii}=\mathbb{E}[(x_{i}^{> \tau})^{2}]$$
2. 
3. $\mathbb{E}[(w_{1}w_{1}^\top)_{ii}]=\mathbb{E}[(x_{i}^{>\tau})^{2}]=\mathbb{E}[(x_{1}^{>\tau})^{2}]=\mathbb{E}[(w_{1}w_{1}^\top)_{11}]\geq 0$. 
   
   Let $X:=\mathbb{E}[w_{1}w_{1}^\top]$. Then, one sees that $X\succeq 0$. Indeed, $$z^\top Xz=\mathbb{E}[zw_{1}w_{1}^\top z]\geq 0,\quad \forall z$$Further, as $X_{11}\geq 0$, $\frac{1}{X_{11}}X\succeq 0$ and $\text{diag}(\frac{1}{X_{11}}X)=I_{2n}$. Therefore we have that: $$\mathbb{E}[\braket{ x^{>\tau} ,Ay^{\leq \tau}  } ]=\mathbb{E}\left[ \left\langle w_{1}w_{1}^\top , \begin{bmatrix}0&A\\0&0\end{bmatrix} \right\rangle \right]= \left\langle X , \begin{bmatrix}0&A\\0&0\end{bmatrix} \right\rangle= X_{11}\left\langle \frac{1}{X_{11}} X , \begin{bmatrix}0&A\\0&0\end{bmatrix} \right\rangle\leq X_{11}\left\| A \right\| _{G}$$Analogously it holds for $w_{2},w_{3}$ and we have our statement. 
2. We claim that a sufficient condition is $\alpha\geq 1$ and $\alpha\beta=1$. Let $X_{1}:=\mathbb{E}[w'_{1}w'^\top_{1}]$ and $X_{2}:=\mathbb{E}[w'_{2}w'^\top_{2}]$. Then similarly to above, $$(X_{1}+X_{2})_{ii}=\begin{cases}\alpha^{2}\mathbb{E}[(x_{1}^{> \tau})^{2}]\end{cases}$$
   
   We have that: $$\mathbb{E}[w'_{1}w'^\top_{1}]+\mathbb{E}[w'_{2}w'^\top_{2}]$$



---
1. We claim that $\alpha\beta=1$ is a sufficient condition. Let $\alpha\beta=1$. Then, $$\mathbb{E}[(x_{1}^{> r})^{2}]=$$
   
   We have that: $$(\alpha^{2}-1)\mathbb{E}[(x^{>r}_{1})^{2}]-\left(1- \frac{1}{\alpha^{2}}\right)\mathbb{E}[(x_{1}^{\leq r})^{2}]\geq 0$$ $$\mathbb{E}[(x^{>r}_{1})^{2}]\geq \frac{1}{\alpha^{2}}\mathbb{E}[(x_{1}^{\leq r})^{2}]$$Notice that: $$\begin{aligned}\mathbb{E}[(x^{>r}_{1})^{2}]=\mathbb{E}[(x_{1}-x^{\leq \tau}_{1})^{2}]=1-2\mathbb{E}[x_{1}x_{1}^{\leq \tau}]+\mathbb{E}[(x_{1}^{\leq \tau})^{2}]\end{aligned}$$where: $$\mathbb{E}[x_{1}x_{1}^{\leq \tau}]=\int_{-\tau}^{\tau} x^2\gamma(x) \, dx +2\tau\int_{\tau}^{\infty} x\gamma(x) \, dx$$
   
3. From 1, we have that: $$\mathbb{E}[\braket{ x^{> \tau} , Ay^{\leq \tau} } +\braket{ x^{\leq \tau} ,Ay^{> \tau}  } ]\leq \mathbb{E}[w_{1}w_{1}^\top+w_{2}w_{2}^\top]_{11}\left\| A \right\| _{G}$$Hence, a sufficient condition is if $$\mathbb{E}[(x_{1}^{>\tau})^{2}]+\mathbb{E}[(x^{\leq \tau}_{1})^{2}]=\mathbb{E}[w_{1}w_{1}^\top+w_{2}w_{2}^\top]_{11}\leq \mathbb{E}[w'_{1}(w'_{1})^\top+w'_{2}(w'_{2})^\top]_{11} =\alpha^{2}\mathbb{E}[(x_{1}^{>\tau})^{2}]+\beta^{2}\mathbb{E}[(x^{\leq \tau}_{1})^{2}]$$

4. We have that: $$\mathbb{E}[w'_{1}(w'_{1})^\top]_{ii}=\beta^{2}\mathbb{E}[(x_{i}^{\leq \tau})^{2}]=\beta^{2}\left( \int_{-\tau}^{\tau} x^{2}\gamma(x) \, dx +2\tau^{2}\int_{\tau}^{\infty} \gamma(x) \, dx \right) $$for $\gamma(x)$ as the standard Gaussian density. Then, $$\int_{\tau}^{\infty}  \gamma(x)\, dx=\int_{\tau}^{\infty} \frac{ \gamma(x)}{\gamma(x-\tau)}\gamma(x-\tau)\, dx\leq\sup_{x\geq \tau}\frac{ \gamma(x)}{\gamma(x-\tau)}\int_{0}^{\infty} \gamma(x) \, dx=\frac{1}{2} e^{-\tau^{2} / 2} $$