#Series #Algorithms 

#### Part 1. Degree concentration
Let $H=(V,E)$ be any undirected graph. We first claim that $d(H)=2\left| E \right| / \left| V \right|$. Indeed, from the handshake lemma, $$\left| E \right| =\frac{1}{2}\sum_{v\in V}^{}d(v)=\frac{1}{2}d(G)\left| V \right| $$

Now, for $G\sim G\left( n, \frac{d}{n} \right)$. For any edge $e\in E(K_{n})$, et $X_{e}=\mathbb{1}_{e\in E(G)}$. By definition, $X_{e}\sim \text{Ber}( d /n)$ i.i.d. Now from the above claim, $d(G)=\frac{2}{n}X$ where $X:=\sum_{e}^{}X_{e}$. Further, we have that $\mathbb{E}[X]=\sum_{e}^{} \frac{d}{n}=\frac{n-1}{2}\cdot d$. Therefore, for $\varepsilon:=20\sqrt{ \frac{d\log n}{n} }$. $$\begin{aligned}\mathbb{P}\left( \left| d(G)-d \right| \geq  \varepsilon\right)&=\mathbb{P}\left( \left| \frac{2}{n}X-\frac{2}{n-1}\mathbb{E}[X] \right| \geq  \varepsilon \right)\leq \mathbb{P}\left( \left| \frac{2}{n}X-\frac{2}{n}\mathbb{E}[X] \right| \geq  \varepsilon\right)\\&\leq \mathbb{P}\left( \left| X-\mathbb{E}[X] \right| \geq \frac{\varepsilon n}{2}\right)\leq \mathbb{P}\left( \left| X-\mathbb{E}[X] \right| \geq \frac{\varepsilon}{d} \frac{ n}{n-1}\mathbb{E}[X]\right)\end{aligned}$$where $\frac{\varepsilon}{d}\frac{n}{n-1}=\frac{20}{n-1} \sqrt{ \frac{n\log n}{d} }<1$ as $d\geq C\log n$ for large enough constant. Hence, by Chernoff, $$\mathbb{P}(\left| d(G)-d \right| \geq \varepsilon)\leq 2\exp\left( -\frac{400}{6} \frac{n}{n-1}\log n\right)\leq n^{-10} $$

---
#### Part 2. Spectral norm bound
From Part 1, we have that with probability $\geq 1-n^{-10}$, we have from $d\geq C\log n$ that: $$d\leq d(G)+20\sqrt{ \frac{d}{n}\log n }\leq d(G)+\frac{20}{\sqrt{ Cn }}d$$Assuming $C$ is large enough, we may wlog assume that $\frac{20}{\sqrt{ Cn }}\leq \frac{1}{20}$. Therefore, $d\leq \frac{20}{19}d(G)$. Now, 
$$\overline{G}=G-\mathbb{E}[G]+\mathbb{E}[G]-\frac{d(G)}{n}11^\top=G-\mathbb{E}[G]+\frac{d-d(G)}{n}11^\top-\frac{d}{n}I_{n}$$We first bound the spectrum of $\frac{d-d(G)}{n}11^\top-\frac{d}{n}I_{n}$. Let $0< \alpha < 1 / n$. Then, as $\text{Spec}(\alpha 11^\top)=\{ \alpha n,0 \}$, we have that: $\left\| I-\alpha 11^\top \right\| =\max\{1-\alpha n,1 \}=1$. Indeed, $\lambda$ is an eigenvalue of $\alpha 11^\top$, if and only if $1-\lambda$ is an eigenvalue for $I-\alpha 11^\top$.

 
Therefore, as we have that $\frac{d-d(G)}{d}\leq \frac{20}{\sqrt{ Cn }}\leq \frac{1}{20}$ from above, we have that:$$\left\| \frac{d-d(G)}{n}11^\top-\frac{d}{n}I_{n} \right\| =\frac{d}{n}\left\| I_{n}-\frac{d-d(G)}{d}11^\top \right\|=\frac{d}{n} \leq 1\leq \sqrt{ d\log n }$$To bound the spectrum of $G-\mathbb{E}[G]$, we use the matrix Bernstein inequality: We have: $$G-\mathbb{E}[G]=\sum_{i<j}Z^{ij},\quad Z^{ij}:=\left( X_{ij}- \frac{d}{n} \right)(E_{ij}+E_{ji})$$where $E^{ij}$ is the indicator matrix at $(i,j)$ and $X_{ij}$ is the indicator variable from above. Then, $Z^{ij}$ is symmetric and zero-mean by definition and: $$\left\| Z^{ij} \right\| =\left| X_{ij}-\frac{d}{n} \right| \left\| E_{ij}+E_{ji} \right\| =\left| X_{ij}-\frac{d}{n} \right| \leq 1$$Further, $$\mathbb{E}[(Z^{ij})^{2}]=\left( \underbrace{ \mathbb{E}[X_{ij}^{2}] }_{ \frac{d}{n}\left( 1-\frac{d}{n} \right) }-\frac{d^{2}}{n^{2}} \right)(E_{ii}+E_{jj})=\frac{d}{n}(E_{ii}+E_{jj})$$Therefore, $$\left\| \sum_{i<j}^{}\mathbb{E}[(Z^{ij})^{2}] \right\| =\left\| \frac{d}{n}(n-1)I_{n} \right\| =\frac{d(n-1)}{n}\leq d$$It follows that with probability $1-n^{-10}$, $$\left\| G-\mathbb{E}[G] \right\| \leq 8(\sqrt{ d \log n }+\log n)\leq 8\left( 1+\frac{1}{\sqrt{ C }} \right)\sqrt{ d\log n }$$By assuming $C$ is large enough, we may assume that $8\left( 1+\frac{1}{\sqrt{ C }} \right)\leq \frac{17}{2}$. Bringing it all together, 

$$\left\| \overline{G} \right\| \leq \left\| G-\mathbb{E}[G] \right\|+\left\| \mathbb{E}[G]-\frac{d(G)}{n} 11^\top \right\| \leq \frac{19}{2}\sqrt{ d\log n }\leq 10\sqrt{ d(G)\log n } $$with error probability at most $2n^{-10}\leq n^{-9}$ using union bound. As $\overline{G}$ is symmetric, we also have that: $\left\| \overline{G}^{2} \right\| =\left\| \overline{G} \right\| ^{2}\leq 100d(G) \log n$.

---
#### Part 3. Median fails
Let $G\sim G(n, d /n)$. We construct an adversary as follows. Let $d_{\text{med}}$ be the median of $G$. 
1. If $\left| d_{\text{med}}-d \right|\geq 0.99\eta n$, then the adversary does nothing and $G':= G$.
2. If $0\leq d_{\text{med}}-d< 0.99\eta n$, then the adversary finds the $\left\lfloor\eta n\right\rfloor$ vertices in $G$ with the lowest degree and adds all possible edges incident to them.
3. If $0\leq d-d_{\text{med}}< 0.99\eta n$, then the adversary finds the $\eta n$ vertices in $G$ with the highest degree and deletes all edges incident to them.

Assume that $d\leq d_{\text{med}}<d+ 0.99 \eta n$ (Case 2). Then, for each of the $\eta n$ vertices, we increase the degree by at least $(n-1-d_{\text{med}})$. Therefore, the total increase of the degrees is at least $(n-1-d_{\text{med}})\eta n$. 

We have that:
1. $\frac{n}{2}d_{\text{med}}\leq \sum_{i}^{}\text{deg}_{G}(i)\leq \frac{n}{2}(d_{\text{med}}+n-1)$
2. $\frac{n}{2}(\widehat{d}_{\text{med}}+\eta n)\leq \sum_{i}^{}\text{deg}_{G'}(i)\leq \frac{n}{2}(\widehat{d}_{\text{med}}+n-1)$
3. $\delta(G')\geq \eta n$

Therefore, $$\frac{n}{2}(\widehat{d}_{\text{med}}+n-1-d_{\text{med}})\geq\sum_{i}^{}\text{deg}_{G'}(i)-\deg_{G}(i)\geq \eta n(n-1-d_{\text{med}})$$

Hence, $\widehat{d}_{\text{med}}+n-1-d\geq \widehat{d}_{\text{med}}+n-1-d_{\text{med}}\geq 2\eta (n-1-d_{\text{med}})$.$$\widehat{d}_{\text{med}}-d\geq  (1-0.99\eta)2\eta n-2\eta-n+1-2\eta d$$

$$\widehat{d}_{\text{med}}\geq \left( 2\eta-1\right)(n-1-d_{\text{med}})\overset{ ? }{ \geq }d+0.99\eta n$$$$$$


Let $d_{\text{med}}$ be the median of $G$. Further, let $d_{\text{low}}, d_{\text{high}}$ be the $\left( \frac{1}{2}-\eta \right)n$ and $\left( \frac{1}{2}+\eta \right)n$ smallest degree of $G$, respectively.
1. If ${d}_{\text{med}}< d$, then the adversary finds the $\eta n$ vertices in $G$ with the lowest degree and adds all possible edges incident to them.
2. If ${d}_{\text{med}}\geq d$, 

Let $G'$ denote the modified graph. Then, as $\text{deg}_{G'}(1),\dots,\deg_{G'}(n)$ differ from $\text{deg}_{G}(1),\dots,\deg_{G}(n)$ in at most $\eta n$ nodes, we have that $d_{\text{low}}\leq\widehat{d}_{\text{med}}\leq d_{\text{high}}$. 
1. If $d_{\text{med}}< d$, then

---
#### Part 4. Spectral certificate
Let $Y$ be a $\rho$-node corruption of $G$. Then, there exists $S\subseteq[n]$ s.t. $\left| S \right|\geq (1-\rho) n$ and for all $i,j\in S$ $Y_{ij}=G_{ij}$. Therefore, in otherwords, we have: $\braket{ G-Y , 1_{S}1_{S}^\top }=0$. It follows that,$$\begin{aligned}\left| d(G)-d(Y) \right| &=\frac{1}{n}\left| \braket{ G-Y , 11^\top }  \right| \\&=\frac{1}{n}\left| \braket{ G-Y , 11^\top -1_{S}1_{S}^\top}  \right| \\&=\frac{1}{n}\left| \left\langle \overline{G}-\overline{Y}+\frac{d(G)-d(Y)}{n}11^\top , 11^\top -1_{S}1_{S}^\top\right\rangle  \right|\\&\leq\frac{1}{n}\left| \left\langle \overline{G}-\overline{Y},11^\top -1_{S}1_{S}^\top\right\rangle \right|+\frac{\left| d(G)-d(Y) \right| }{n^{2}}\left|\left\langle 11^\top , 11^\top -1_{S}1_{S}^\top\right\rangle  \right| \end{aligned}$$
Now, $$\braket{ 11^\top  , 11^\top -1_{S}1_{S}^\top } =n^2-\left| S \right| ^{2}\leq (1-(1-\rho)^{2})n^{2}$$Further, by defining $\overline{S}:=[n] \backslash S$, we have: $$11^\top-1_{S}1_{S}^\top=1_{S}1_{\overline{S}}^\top+1_{\overline{S}}1_{S}^\top+1_{\overline{S}}1_{\overline{S}}^\top$$Therefore, $$\begin{aligned}\left| \braket{ \overline{G}-\overline{Y} , 11^\top-1_{S}1_{S}^\top }  \right| &\leq \left\| \overline{G}-\overline{Y} \right\| \left\| 11^\top-1_{S}1_{S}^\top \right\| _{*}\leq \left\| \overline{G}-\overline{Y} \right\| \left(2 \left\| 1_{S}1_{\overline{S}}^\top \right\| _{*}+ \left\| 1_{\overline{S}}1_{\overline{S}}^\top \right\| _{*}\right) \end{aligned}$$where as $1_{S}1_{\overline{S}}^\top$ and $1_{\overline{S}}1_{\overline{S}}^\top$ are both rank 1, $$\left\| 1_{S}1_{\overline{S}}^\top \right\| _{*}\leq \left\| 1_{S}1_{\overline{S}}^\top \right\| _{F}=\sqrt{ \text{tr}(1_{S}^\top1_{S}1_{\overline{S}}^\top 1_{\overline{S}} ) }=\sqrt{ \left| S \right| (n-\left| S \right| ) }\leq \sqrt{ n }\sqrt{ \rho n }=\sqrt{ \rho }n$$Similarly, $\left\| 1_{\overline{S}}1_{\overline{S}}^\top \right\|_{*}\leq n-\left| S \right|\leq \rho n\leq \sqrt{ \rho }n$ as $\rho\leq 1$. Therefore, $$2 \left\| 1_{S}1_{\overline{S}}^\top \right\| _{*}+ \left\| 1_{\overline{S}}1_{\overline{S}}^\top \right\| _{*}\leq 3\sqrt{ \rho }n $$Now, as $\rho\leq c$ for some constant $c$, we have that: $$(1-c)^{2}\left| d(G)-d(Y) \right| \leq (1-\rho)^{2}\left| d(G)-d(Y) \right| \leq 3\sqrt{ \rho }\left\| \overline{G}-\overline{Y} \right\|\leq 3\sqrt{ \rho }\left( \left\| \overline{G} \right\| +\left\| \overline{Y} \right\|  \right)  $$we have the desired statement.


---
#### Part 5. Using spectral certificates inside SOS
Using $\vdash \braket{ a , b }\leq\|a\|^{2}\|b\|^{2}$ from 8. Useful SOS Proofs,  $$\begin{aligned}\{ M=M^\top,M^2=\alpha I_{n}- RR^\top \}\vdash \braket{ x , My } ^{2}&\leq \|x\|^{2}\|My\|^{2}\\&=\|x\|^{2} y^\top M^\top My\\&=\|x\|^{2} y^\top M^{2}y\\&=\|x\|^{2} y^\top (\alpha I_{n}-RR^\top)y\\&=\alpha\|x\|^{2}\|y\|^{2}-\|x\|^{2}\|R^\top y\|^{2}\\&\leq \alpha\|x\|^{2}\|y\|^{2}\end{aligned}$$where the last inequality follows as $\|x\|^2\|R^\top y\|^{2}$ is a square. We also see that the degree is constant. 

---
#### Part 6. SoS identifiability, Part I
As we have that $$\mathcal{A}\vdash Y_{ij}\tilde{z}_{i}\tilde{z}_{j}=G_{ij}\tilde{z}_{i}\tilde{z}_{j},\quad \forall i,j\in[n]$$it follows that:
$$\begin{aligned}\mathcal{A}\vdash n(d(Y)-d(G))&=\braket{Y- G , 11^\top }\\&=\braket{Y- G , 11^\top -\tilde{z}\tilde{z}^\top} \\&=\left\langle\overline{Y}- \overline{G} +\frac{d(Y)-d(G)}{n}11^\top , 11^\top -\tilde{z}\tilde{z}^\top\right\rangle \\&=\braket{ \overline{Y} , 11^\top-\tilde{z}\tilde{z}^\top } -\braket{ \overline{G} , 11^\top-\tilde{z}\tilde{z}^\top } +\frac{d(Y)-d(G)}{n}\braket{11^\top , 11^\top-\tilde{z}\tilde{z}^\top } \\&=\braket{ \overline{Y} , 11^\top-\tilde{z}\tilde{z}^\top } -\braket{ \overline{G} , 11^\top-\tilde{z}\tilde{z}^\top } +n\left( 1-\left( \frac{\braket{ \tilde{z} , 1 } }{n} \right)^{2} \right)(d(Y)-d(G))\end{aligned} $$where the last step follows from:$$\braket{ 11^\top , 11^\top -\tilde{z} \tilde{z}^\top } =n^2-\sum_{i,j}^{}\tilde{z}_{i}\tilde{z}_{j}=n^2-\braket{ \tilde{z} , 1 } ^{2}=n^2\left( 1-\left( \frac{\braket{ \tilde{z} , 1 } }{n} \right)^{2}  \right) $$Therefore, by rearranging:
$$\mathcal{A}\vdash n\left( \frac{\braket{ \tilde{z} , 1 } }{n} \right)^{2}(d(Y)-d(G))=\braket{ \overline{Y} , 11^\top-\tilde{z}\tilde{z}^\top } -\braket{ \overline{G} , 11^\top-\tilde{z}\tilde{z}^\top } $$By squaring both sides, $$\begin{aligned}\mathcal{A}\vdash n^{2}(d(Y)-d(G))^{2}&= \left( \frac{n}{\braket{ \tilde{z} , 1 } }\right)^{4}(\braket{ \overline{Y} , 11^\top-\tilde{z}\tilde{z}^\top } -\braket{ \overline{G} , 11^\top-\tilde{z}\tilde{z}^\top } )^{2}\\&\le 2 \left( \frac{n}{\braket{ \tilde{z} , 1 } }\right)^{4}(\braket{ \overline{Y} , 11^\top-\tilde{z}\tilde{z}^\top }^{2} +\braket{ \overline{G} , 11^\top-\tilde{z}\tilde{z}^\top }^{2} )\end{aligned}$$Now it suffices to show that $\frac{n}{\braket{ \tilde{z} , 1 }}\leq O(1)$.  We have that: $$\mathcal{A}\vdash n\leq \frac{1}{1-2\eta}\braket{ \tilde{z} , 1 } \leq \frac{1}{1-\frac{2}{C}}\braket{ \tilde{z} , 1 } =O(1)\braket{ \tilde{z} , 1 } $$

---
#### Part 7. SoS identifiability, Part II
Let $\tilde{w}:=1-\tilde{z}$. Then, $$\begin{aligned}\mathcal{A}\vdash \tilde{w} \tilde{z}^\top+\tilde{z} \tilde{w}^\top+\tilde{w}\tilde{w}^\top&=1\tilde{z}^\top-\tilde{z}\tilde{z}^\top+\tilde{z} 1^\top - \tilde{z} \tilde{z}^\top+1 1^\top -1\tilde{z}^\top-\tilde{z} 1^\top+\tilde{z}\tilde{z}^\top\\&=1 1^\top -\tilde{z}\tilde{z}^\top\end{aligned}$$Therefore, $$\begin{aligned}\mathcal{A}\vdash \braket{ \overline{Y} , 11^\top-\tilde{z} \tilde{z}^\top }  ^{2} &=\braket{ \overline{Y} , \tilde{w}\tilde{z}^\top+\tilde{z}\tilde{w}^\top+\tilde{w}\tilde{w}^\top }  ^{2}\\ &=(\braket{ \tilde{z} , \overline{Y} \tilde{w} }+\braket{ \tilde{w} , \overline{Y} \tilde{z} } +\braket{ \tilde{w} , \overline{Y} \tilde{w} })^{2}\\ &=(2\braket{ \tilde{z} , \overline{Y} \tilde{w} } +\braket{ \tilde{w} , \overline{Y} \tilde{w} })^{2}\\ &\leq 4\braket{ \tilde{z} , \overline{Y} \tilde{w} }^{2} +\braket{ \tilde{w} , \overline{Y} \tilde{w} }^{2}\end{aligned}$$Now, as $Y=Y^\top$ we have that $\overline{Y}=\overline{Y}^\top$ under $\mathcal{A}$ and therefore, using Part 5, we have that: $$\mathcal{A}\vdash \braket{ x , \overline{Y}y }^{2}\leq 100 d(Y)\log n\|x\|^{2}\|y\|^{2}$$Therefore, $$\mathcal{A}\vdash \braket{ \overline{Y} , 11^\top-\tilde{z} \tilde{z}^\top } ^{2}\leq 400 d(Y)\log n \|\tilde{z}\|^{2}\|\tilde{w}\|^{2}+100d(Y)\log n \|\tilde{w}\|^4$$where: $$\mathcal{A}\vdash \left\| \tilde{w} \right\| ^{2}=\sum_{i}^{}(1-\tilde{z}_{i})^{2}=\sum_{i}^{}1-2\tilde{z}_{i}+\tilde{z}^{2}_{i}=\sum_{i}^{}1-\tilde{z}_{i}\leq 2\eta n$$Lastly, as we have $\mathcal{A}\vdash \tilde{z}^{2}_{i}= \tilde{z}_{i}$ for all $i$, we have that $\mathcal{A}\vdash \tilde{z}_{i}\leq 1$. Therefore,$$\mathcal{A}\vdash \|\tilde{z}\|^{2}=\sum_{i}^{}\tilde{z}_{i}^{2}=\sum_{i}^{}\tilde{z}_{i}\leq \sum_{i}1=n$$Bringing everything together, $$\mathcal{A}\vdash \braket{ \overline{Y} , 11^\top-\tilde{z} \tilde{z}^\top } ^{2}\leq 800 \eta n^{2} \log n \cdot d(Y)  +400 \eta^{2} n^{2}\log n \cdot d(Y)=O(\eta n^{2} \log n)d(Y)$$as $\eta\leq 1$.

---
#### Part 8. Final estimation guarantee
We have that: $$\begin{aligned}\mathcal{A}\vdash (d(Y)-d(G))^{2}&\leq O\left( \frac{1}{n^{2}} \right)\left( \braket{ \overline{G} , 11^\top-\tilde{z}\tilde{z}^\top } ^{2}+\braket{ \overline{Y} , 11^\top-\tilde{z}\tilde{z}^\top } ^{2} \right)\\&\leq O\left(\eta \log n\right)(d(G)+d(Y))\\&\leq D\eta \log n(d(G)+d(Y))\end{aligned} $$ for some constant $D$. 


Now, $$\begin{aligned}\mathcal{A}\vdash d(Y)&=\frac{d(Y)-d(G)}{\sqrt{ D\eta \log n }}\sqrt{ D\eta \log n }+d(G)\\&\leq \frac{(d(Y)-d(G))^{2}}{2D\eta \log n}+d(G)+\frac{D}{2}\eta \log n\\&\leq \frac{(d(Y)-d(G))^{2}}{2D\eta \log n}+O(1)d(G)\end{aligned}$$where $O(1)$ comes from the fact that $\eta \log n\leq \frac{d}{C^{2}}$ and $d\leq O(1)d(G)$ with probability at least $1-n^{-9}$ together with $\mathcal{A}_{\text{goodness}}$ (cf. Part 2). Therefore, $$\begin{aligned}\mathcal{A}\vdash (d(Y)-d(G))^{2}&\leq D\eta \log n\left( O(1)d(G)+\frac{(d(Y)-d(G))^{2}}{2D\eta \log n}\right) \\&=\frac{(d(Y)-d(G))^{2}}{2}+ O(\eta \log n)d(G)\end{aligned}$$Rearranging the statement we have that $\mathcal{A}\vdash (d(Y)-d(G))^2\leq O(\eta \log n)d(G)$.

Now, by the SOS meta theorem and the fact that $d(Y)=\frac{1}{n}\braket{ Y , 11^\top }$, we have that: $$(\widehat{d}-d(G))^{2}=\left( \frac{1}{n}\braket{ \tilde{\mathbb{E}}[Y] , 11^\top }  -d(G)\right)^{2}\leq O(\eta \log n)d(G)\leq O(\eta \log n \cdot d)$$Therefore, with Part 1, with probability at least $1-n^{-5}$: $$\left| \widehat{d}-d \right| \leq \left| \widehat{d}-d(G) \right| +\left| d(G)-d \right| \leq O\left( \sqrt{ \frac{d\log n}{n} }+ \sqrt{ \eta \log n \cdot d }\right)$$

---
